Fix translation of struct pointers
This makes the code a bit ad-hoc in places; ideally the support for
structs would be more obvious and systematic, but it's kind of
fundamental that we now treat struct pointers unlike generic pointers to
struct values, and most of the complexity is still handled in Coq (goose
just checks if something is a struct and uses a more normal translation
if it's not).

goose.go
@@ -247,6 +247,10 @@ func (ctx Ctx) ptrType(e *ast.StarExpr) coq.Type {
 			return coq.TypeIdent("lockRefT")
 		}
 	}
+	name, _, ok := getStructType(ctx.typeOf(e.X))
+	if ok {
+		return coq.NewCallExpr("struct.ptrT", coq.StructDesc(name))
+	}
 	return coq.PtrType{ctx.coqType(e.X)}
 }
 
@@ -544,11 +548,11 @@ func (ctx Ctx) newExpr(s ast.Node, ty ast.Expr) coq.CallExpr {
 			return coq.NewCallExpr("Data.newLock")
 		}
 	}
+	e := coq.NewCallExpr("zero_val", ctx.coqType(ty))
 	if _, _, ok := getStructType(ctx.typeOf(ty)); ok {
-		// TODO: should be flattening struct across multiple addresses
+		return coq.NewCallExpr("struct.alloc", e)
 	}
-	return coq.NewCallExpr("ref",
-		coq.NewCallExpr("zero_val", ctx.coqType(ty)))
+	return coq.NewCallExpr("ref", e)
 }
 
 // basicallyUInt64 returns true conservatively when an
@@ -629,6 +633,16 @@ func getStructType(t types.Type) (string, *types.Struct, bool) {
 		}
 	}
 	return "", nil, false
+}
+
+// TODO: unify getStructType and getStructPointerType and have them return a
+//  struct of struct type info
+func getStructPointerType(t types.Type) (string, bool) {
+	if t, ok := t.(*types.Pointer); ok {
+		name, _, ok := getStructType(t.Elem())
+		return name, ok
+	}
+	return "", false
 }
 
 func (ctx Ctx) selectExpr(e *ast.SelectorExpr) coq.Expr {
@@ -1278,6 +1292,13 @@ func (ctx Ctx) assignStmt(s *ast.AssignStmt, c *cursor, loopVar *string) coq.Bin
 			ctx.unsupported(s, "index update to unexpected target of type %v", targetTy)
 		}
 	case *ast.StarExpr:
+		name, ok := getStructPointerType(ctx.typeOf(lhs.X))
+		if ok {
+			return coq.NewAnon(coq.NewCallExpr("struct.store",
+				coq.StructDesc(name),
+				ctx.expr(lhs.X),
+				ctx.expr(s.Rhs[0])))
+		}
 		return coq.NewAnon(coq.StoreStmt{
 			Dst: ctx.expr(lhs.X),
 			X:   ctx.expr(s.Rhs[0]),
@@ -1287,10 +1308,9 @@ func (ctx Ctx) assignStmt(s *ast.AssignStmt, c *cursor, loopVar *string) coq.Bin
 		if ty, ok := ty.(*types.Pointer); ok {
 			name, _, ok := getStructType(ty.Elem())
 			if ok {
-				structDesc := fmt.Sprintf("%s.S", name)
 				fieldName := lhs.Sel.Name
 				return coq.NewAnon(coq.NewCallExpr("struct.storeF",
-					coq.GallinaIdent(structDesc),
+					coq.StructDesc(name),
 					coq.GallinaString(fieldName),
 					ctx.expr(lhs.X),
 					ctx.expr(rhs)))
