internal/examples/mailserver/mailserver.gold.v
@@ -14,7 +14,6 @@ Module partialFile.
   Section fields.
     Context `{ext_ty: ext_types}.
     Definition get := struct.get S.
-    Definition loadF := struct.loadF S.
   End fields.
 End partialFile.
 
@@ -63,7 +62,6 @@ Module Message.
   Section fields.
     Context `{ext_ty: ext_types}.
     Definition get := struct.get S.
-    Definition loadF := struct.loadF S.
   End fields.
 End Message.
 
