internal/examples/wal/wal.gold.v
@@ -20,7 +20,6 @@ Module Log.
   Section fields.
     Context `{ext_ty: ext_types}.
     Definition get := struct.get S.
-    Definition loadF := struct.loadF S.
   End fields.
 End Log.
 
